theories/stenning.v
@@ -162,7 +162,7 @@ Section stenning_ex.
     iDestruct (ltl_now_prod_fst with "Hs") as (stB) "Hs".
     iDestruct (ltl_now_label_prod_fst with "HA") as (l) "HA".
     iDestruct (ltl_dup with "HA") as "[HA HA']".
-    iDestruct (trace_steps_det with "[Hs HA]") as  (s' Hsteps') "Hs'".
+    iDestruct (trace_steps_label with "[Hs HA]") as  (s' Hsteps') "Hs'".
     { eexists _,_. econstructor. }
     { iFrame. }
     inversion Hsteps'; simplify_eq.
@@ -181,7 +181,7 @@ Section stenning_ex.
     iDestruct (ltl_now_prod_fst with "Hs") as (stB) "Hs".
     iDestruct (ltl_now_label_prod_fst with "HA") as (l) "HA".
     iDestruct (ltl_dup with "HA") as "[HA HA']".
-    iDestruct (trace_steps_det with "[$Hs $HA]") as  (s' Hsteps') "Hs'".
+    iDestruct (trace_steps_label with "[$Hs $HA]") as  (s' Hsteps') "Hs'".
     { eexists (_,Recv _ None),_. econstructor. eauto. }
     inversion Hsteps'; simplify_eq.
     - iExists omsg. iLeft. iFrame. iSplit; [eauto|]. iModIntro.
@@ -197,7 +197,7 @@ Section stenning_ex.
     iDestruct (ltl_now_prod_fst with "Hs") as (stB) "Hs".
     iDestruct (ltl_now_label_prod_fst with "HA") as (l) "HA".
     iDestruct (ltl_dup with "HA") as "[HA HA']".
-    iDestruct (trace_steps_det with "[$Hs $HA]") as  (s' Hsteps') "Hs'".
+    iDestruct (trace_steps_label with "[$Hs $HA]") as  (s' Hsteps') "Hs'".
     { apply stenning_reducible. }
     inversion Hsteps'; simplify_eq;
       iModIntro; iApply ltl_now_prod_fst; iExists _; iFrame.
@@ -214,7 +214,7 @@ Section stenning_ex.
     iDestruct (ltl_now_prod_snd with "Hs") as (stA) "Hs".
     iDestruct (ltl_now_label_prod_fst with "Hl") as (l) "Hl".
     iDestruct (ltl_dup with "Hl") as "[Hl Hl']".
-    iDestruct (trace_steps_det with "[$Hs $Hl]") as  (s' Hsteps') "Hs'".
+    iDestruct (trace_steps_label with "[$Hs $Hl]") as  (s' Hsteps') "Hs'".
     { apply stenning_reducible. }
     inversion Hsteps'; simplify_eq.
     - iExists None. iLeft. iFrame. iSplit; [eauto|]. iModIntro.
@@ -232,7 +232,7 @@ Section stenning_ex.
     iDestruct (ltl_now_prod_snd with "Hs") as (stA) "Hs".
     iDestruct (ltl_now_label_prod_fst with "Hl") as (l) "Hl".
     iDestruct (ltl_dup with "Hl") as "[Hl Hl']".
-    iDestruct (trace_steps_det with "[$Hs $Hl]") as  (s' Hsteps') "Hs'".
+    iDestruct (trace_steps_label with "[$Hs $Hl]") as  (s' Hsteps') "Hs'".
     { apply stenning_reducible. }
     inversion Hsteps'; simplify_eq.
     iFrame. iModIntro. iApply ltl_now_prod_snd. iExists _. iFrame.
@@ -245,7 +245,7 @@ Section stenning_ex.
     iDestruct (ltl_now_prod_snd with "Hs") as (stA) "Hs".
     iDestruct (ltl_now_label_prod_fst with "Hl") as (l) "Hl".
     iDestruct (ltl_dup with "Hl") as "[Hl Hl']".
-    iDestruct (trace_steps_det with "[$Hs $Hl]") as  (s' Hsteps') "Hs'".
+    iDestruct (trace_steps_label with "[$Hs $Hl]") as  (s' Hsteps') "Hs'".
     { apply stenning_reducible. }
     inversion Hsteps'; simplify_eq;
       iModIntro; iApply ltl_now_prod_snd; iExists _; iFrame.
